Local_Rules.thy
@@ -1,96 +1,17 @@
 theory Local_Rules
-  imports Syntax
+  imports Atomics
 begin
 
 chapter \<open>Local Rules\<close>
 
 text \<open>Define the rely/guarantee rules for a local program.\<close>
 
-section \<open>Helper Definitions\<close>
-
-text \<open>Stability of a predicate across an environment step\<close>
-definition stable :: "'a rel \<Rightarrow> 'a set \<Rightarrow> bool"
-  where "stable R P \<equiv> \<forall>m m'. m \<in> P \<longrightarrow> (m,m') \<in> R \<longrightarrow> m' \<in> P"
-
-text \<open>Weakest precondition for an arbitrary state relation\<close>
-definition wp :: "'b rpred \<Rightarrow> 'b pred \<Rightarrow> 'b pred"
-  where "wp \<alpha> P \<equiv> {m. \<forall>m'. (m,m') \<in> \<alpha> \<longrightarrow> m' \<in> P}"
-
-lemma stable_conseqI [intro]:
-  assumes "stable R' P" "R \<subseteq> R'" 
-  shows "stable R P"
-  using assms rtrancl_mono unfolding stable_def by blast
-
-lemma stable_conjI [intro]:
-  assumes "stable R P" "stable R' P'"
-  shows "stable (R \<inter> R') (P \<inter> P')"
-  using assms by (auto simp: stable_def)
-
-lemma stable_transitive:
-  assumes "(m,m') \<in> R\<^sup>*" "m \<in> P" "stable R P"
-  shows "m' \<in> P"
-  using assms by (induct rule: rtrancl.induct) (auto simp: stable_def)
-
-locale local_rules =
-  fixes eval :: "'a \<Rightarrow> 'b rel" 
+locale local_rules = atomic_rules
 
 context local_rules
 begin
 
-section \<open>Atomic Rule\<close>
-
-text \<open>Weakest precondition for an instruction\<close>
-abbreviation wp\<^sub>\<alpha> :: "'a \<Rightarrow> 'b pred \<Rightarrow> 'b pred"
-  where "wp\<^sub>\<alpha> \<alpha> P \<equiv> wp (eval \<alpha>) P"
-
-text \<open>Specification Check, ensuring an instruction conforms to a relation\<close>
-abbreviation guar :: "'a \<Rightarrow> 'b rpred \<Rightarrow> bool"
-  where "guar \<alpha> G \<equiv> eval \<alpha> \<subseteq> G"
-
-text \<open>Rule for an atomic operation\<close>
-definition atomic_rule :: "'b rpred \<Rightarrow> 'b rpred \<Rightarrow> 'b pred \<Rightarrow> 'a \<Rightarrow> 'b pred \<Rightarrow> bool" 
-  ("_,_ \<turnstile>\<^sub>A _ {_} _" [40,0,0,0,40] 40)
-  where "R,G \<turnstile>\<^sub>A P {\<alpha>} Q \<equiv> P \<subseteq> wp\<^sub>\<alpha> \<alpha> Q \<and> guar \<alpha> G \<and> stable R P \<and> stable R Q"
-
-subsection \<open>Properties\<close>
-
-text \<open>Re-establish an atomic judgement over a stronger stable precondition\<close>
-lemma atomic_pre:
-  assumes "R,G \<turnstile>\<^sub>A P {\<alpha>} Q" "P' \<subseteq> P" "stable R P'"
-  shows "R,G \<turnstile>\<^sub>A P' {\<alpha>} Q"
-  using assms unfolding atomic_rule_def
-  by fast
-
-text \<open>Strengthen the rely and weaken the guarantee for an atomic judgement\<close>
-lemma atomic_conseqI [intro]:
-  assumes "R,G \<turnstile>\<^sub>A P {\<alpha>} Q" "R' \<subseteq> R" "G \<subseteq> G'"
-  shows "R',G' \<turnstile>\<^sub>A P {\<alpha>} Q"
-  using assms unfolding atomic_rule_def
-  by blast
-
-text \<open>Atomic judgements over the same instruction can be combined\<close>
-lemma actomic_conjI [intro]:
-  assumes "R,G \<turnstile>\<^sub>A P\<^sub>1 {\<alpha>} Q\<^sub>1" "R,G  \<turnstile>\<^sub>A P\<^sub>2 {\<alpha>} Q\<^sub>2"
-  shows "R,G \<turnstile>\<^sub>A P\<^sub>1 \<inter> P\<^sub>2 {\<alpha>} Q\<^sub>1 \<inter> Q\<^sub>2"
-  using assms unfolding atomic_rule_def  
-  by (auto simp: wp_def stable_def)
-
-text \<open>Add an invariant across an atomic judgement\<close>
-lemma atomic_frameI [intro]:
-  assumes "R,G \<turnstile>\<^sub>A P {\<alpha>} Q"
-  assumes "stable R\<^sub>2 M" "G \<subseteq> R\<^sub>2"
-  shows "R \<inter> R\<^sub>2,G \<turnstile>\<^sub>A P \<inter> M {\<alpha>} Q \<inter> M"
-  unfolding atomic_rule_def
-proof (safe, goal_cases)
-  case (1 x)
-  hence "{(m,m'). m \<in> P} \<inter> eval \<alpha> \<subseteq> R\<^sub>2" 
-    using assms(1,3) unfolding atomic_rule_def by fast
-  hence "x \<in> wp\<^sub>\<alpha> \<alpha> M" using assms(2) 1 unfolding stable_def wp_def by blast
-  moreover have "x \<in> wp\<^sub>\<alpha> \<alpha> Q" using 1 assms(1) by (auto simp: atomic_rule_def wp_def)
-  ultimately show ?case by (auto simp: wp_def)
-qed (insert assms, auto simp: atomic_rule_def wp_def)
-
-section \<open>Local Rules\<close>
+section \<open>Base Rules\<close>
 
 text \<open>Rules of the logic over a thread, similar to standard Hoare-logic\<close>
 inductive lrules :: "'b rpred \<Rightarrow> 'b rpred \<Rightarrow> 'b pred \<Rightarrow> 'a com \<Rightarrow> 'b pred \<Rightarrow> bool" 
@@ -103,7 +24,7 @@ where
   basic[intro]:  "R,G \<turnstile>\<^sub>A P {\<alpha>} Q \<Longrightarrow> R,G \<turnstile>\<^sub>l P { Basic \<alpha> } Q" |
   conseq[intro]: "R,G \<turnstile>\<^sub>l P { c } Q \<Longrightarrow> P' \<subseteq> P \<Longrightarrow> R' \<subseteq> R \<Longrightarrow> G \<subseteq> G' \<Longrightarrow> Q \<subseteq> Q' \<Longrightarrow> R',G' \<turnstile>\<^sub>l P' { c } Q'"
 
-subsection \<open>Properties\<close>
+section \<open>Derived Properties\<close>
 
 text \<open>
 Various elimination rules based on a judgement over a particular program structure.
