Atomics.thy
@@ -1,0 +1,124 @@
+theory Atomics
+  imports Syntax
+begin
+
+chapter \<open>Atomic Actions\<close>
+
+text \<open>
+Describe concepts the logic must know about atomic instructions. 
+\<close>
+
+section \<open>Helper Definitions\<close>
+
+type_synonym 'b pred = "'b set"
+type_synonym 'b rpred = "'b rel"
+
+text \<open>Stability of a predicate across an environment step\<close>
+definition stable :: "'a rel \<Rightarrow> 'a set \<Rightarrow> bool"
+  where "stable R P \<equiv> \<forall>m m'. m \<in> P \<longrightarrow> (m,m') \<in> R \<longrightarrow> m' \<in> P"
+
+text \<open>Weakest precondition for a precondition and postrelation\<close>
+definition wp 
+  where "wp pre post Q \<equiv> pre \<inter> {m. (\<forall>m'. (m,m') \<in> post \<longrightarrow> m' \<in> Q)}"
+
+text \<open>Weakest precondition of the transitive closure of an arbitrary state relation\<close>
+abbreviation wp\<^sub>t :: "'b rpred \<Rightarrow> 'b pred \<Rightarrow> 'b pred"
+  where "wp\<^sub>t R P \<equiv> wp UNIV (R\<^sup>*) P"
+
+subsection \<open>Helper Lemmas\<close>
+
+lemma stable_conseqI [intro]:
+  assumes "stable R' P" "R \<subseteq> R'" 
+  shows "stable R P"
+  using assms rtrancl_mono unfolding stable_def by blast
+
+lemma stable_conjI [intro]:
+  assumes "stable R P" "stable R' P'"
+  shows "stable (R \<inter> R') (P \<inter> P')"
+  using assms by (auto simp: stable_def)
+
+lemma stable_transitive:
+  assumes "(m,m') \<in> R\<^sup>*" "m \<in> P" "stable R P"
+  shows "m' \<in> P"
+  using assms by (induct rule: rtrancl.induct) (auto simp: stable_def)
+
+lemma stable_wp\<^sub>tI:
+  "stable R P \<Longrightarrow> P \<subseteq> wp\<^sub>t R P"
+  unfolding wp_def using stable_transitive by fast
+
+section \<open>Atomic Properties\<close>
+
+locale atomics =
+  fixes behv :: "'a \<Rightarrow> 'b rel" 
+  and vc :: "'a \<Rightarrow> 'b set"
+
+context atomics
+begin
+
+text \<open>Merge the condition and behaviour to define aborting evaluation\<close>
+definition eval :: "'a \<Rightarrow> 'b rpred"
+  where "eval \<alpha> \<equiv> {(m,m'). m \<in> vc \<alpha> \<longrightarrow> (m,m') \<in> behv \<alpha>}"
+
+text \<open>Weakest precondition for an instruction\<close>
+abbreviation wp\<^sub>\<alpha> :: "'a \<Rightarrow> 'b pred \<Rightarrow> 'b pred"
+  where "wp\<^sub>\<alpha> \<alpha> P \<equiv> wp (vc \<alpha>) (behv \<alpha>) P"
+
+text \<open>Specification Check, ensuring an instruction conforms to a relation\<close>
+abbreviation guar :: "'a \<Rightarrow> 'b rpred \<Rightarrow> bool"
+  where "guar \<alpha> G \<equiv> behv \<alpha> \<subseteq> G"
+
+end
+
+section \<open>Atomic Rule\<close>
+
+locale atomic_rules = atomics
+
+context atomic_rules
+begin
+
+text \<open>Rule for an atomic operation\<close>
+definition atomic_rule :: "'b rpred \<Rightarrow> 'b rpred \<Rightarrow> 'b pred \<Rightarrow> 'a \<Rightarrow> 'b pred \<Rightarrow> bool" 
+  ("_,_ \<turnstile>\<^sub>A _ {_} _" [40,0,0,0,40] 40)
+  where "R,G \<turnstile>\<^sub>A P {\<alpha>} Q \<equiv> P \<subseteq> wp\<^sub>\<alpha> \<alpha> Q \<and> guar \<alpha> G \<and> stable R P \<and> stable R Q"
+
+subsection \<open>Derived Properties\<close>
+
+text \<open>Re-establish an atomic judgement over a stronger stable precondition\<close>
+lemma atomic_pre:
+  assumes "R,G \<turnstile>\<^sub>A P {\<alpha>} Q" "P' \<subseteq> P" "stable R P'"
+  shows "R,G \<turnstile>\<^sub>A P' {\<alpha>} Q"
+  using assms unfolding atomic_rule_def
+  by fast
+
+text \<open>Strengthen the rely and weaken the guarantee for an atomic judgement\<close>
+lemma atomic_conseqI [intro]:
+  assumes "R,G \<turnstile>\<^sub>A P {\<alpha>} Q" "R' \<subseteq> R" "G \<subseteq> G'"
+  shows "R',G' \<turnstile>\<^sub>A P {\<alpha>} Q"
+  using assms unfolding atomic_rule_def
+  by blast
+
+text \<open>Atomic judgements over the same instruction can be combined\<close>
+lemma actomic_conjI [intro]:
+  assumes "R,G \<turnstile>\<^sub>A P\<^sub>1 {\<alpha>} Q\<^sub>1" "R,G  \<turnstile>\<^sub>A P\<^sub>2 {\<alpha>} Q\<^sub>2"
+  shows "R,G \<turnstile>\<^sub>A P\<^sub>1 \<inter> P\<^sub>2 {\<alpha>} Q\<^sub>1 \<inter> Q\<^sub>2"
+  using assms unfolding atomic_rule_def wp_def stable_def
+  by (intro conjI) blast+
+
+text \<open>Add an invariant across an atomic judgement\<close>
+lemma atomic_frameI [intro]:
+  assumes "R,G \<turnstile>\<^sub>A P {\<alpha>} Q"
+  assumes "stable R\<^sub>2 M" "G \<subseteq> R\<^sub>2"
+  shows "R \<inter> R\<^sub>2,G \<turnstile>\<^sub>A P \<inter> M {\<alpha>} Q \<inter> M"
+  unfolding atomic_rule_def
+proof (safe, goal_cases)
+  case (1 x)
+  hence "{(m,m'). m \<in> P} \<inter> behv \<alpha> \<subseteq> R\<^sub>2" "x \<in> vc \<alpha>"
+    using assms(1,3) unfolding atomic_rule_def wp_def by auto
+  hence "x \<in> wp\<^sub>\<alpha> \<alpha> M" using assms(2) 1 unfolding stable_def wp_def by auto
+  moreover have "x \<in> wp\<^sub>\<alpha> \<alpha> Q" using 1 assms(1) by (auto simp: atomic_rule_def wp_def)
+  ultimately show ?case by (auto simp: wp_def)
+qed (insert assms, auto simp: atomic_rule_def wp_def)
+
+end
+
+end
